src/Shallow/ProgLang/ProgTheorems.v
@@ -90,8 +90,7 @@ Proof.
 Qed.
 
 Lemma exec_weaken : forall `(p: prog opT T) `(step: Semantics opT State) (step': Semantics opT State),
-    forall (Hstep: forall T (op: opT T) state v state',
-          step _ op state v state' -> step' _ op state v state'),
+    semantics_impl step step' ->
     forall state r, exec step p state r ->
            exec step' p state r.
 Proof.
